modifies_only_shared_and_encapsulated in default_spec to allow callbacks to modify encapsulated variables

state/Backtranslation.STLCToTargetLang.fst
@@ -197,7 +197,7 @@ val progr_sep_test:
   SST unit
     (requires (fun h0 ->
       satisfy_on_heap rp h0 contains_pred /\
-      ~(is_shared rp h0)))
+      is_private rp h0))
     (ensures (fun h0 _ h1 ->
       sel h0 rp == sel h1 rp)) // the content of rp should stay the same before/ after calling the context
 let progr_sep_test #rp f = (** If this test fails, it means that the spec of f does not give [automatically] separation  **)
@@ -241,7 +241,7 @@ val progr_secret_unchanged_test:
   SST unit
     (requires (fun h0 ->
       satisfy_on_heap rp h0 contains_pred /\
-      ~(is_shared rp h0) /\
+      is_private rp h0 /\
       satisfy_on_heap rs h0 is_shared))
     (ensures (fun h0 _ h1 ->
       sel h0 rp == sel h1 rp))
@@ -258,7 +258,7 @@ val progr_passing_callback_test:
   SST unit
     (requires (fun h0 ->
       satisfy_on_heap rp h0 contains_pred /\
-      ~(is_shared rp h0) /\
+      is_private rp h0 /\
       satisfy_on_heap rs h0 is_shared))
     (ensures (fun h0 _ h1 -> sel h0 rp == sel h1 rp)) // the content of rp should stay the same before/ after calling the context
 // TODO: the callback of the program should be able to modify rp
@@ -273,6 +273,28 @@ let progr_passing_callback_test rp rs f =
   downgrade_val (f cb);
   ()
 
+val progr_passing_callback_test':
+  rp: ref int ->
+  rs: ref (ref int) ->
+  ctx:(elab_typ default_spec (TArr (TArr TUnit TUnit) TUnit)) ->
+  SST unit
+    (requires (fun h0 ->
+      satisfy_on_heap rp h0 contains_pred /\
+      is_private rp h0 /\
+      satisfy_on_heap rs h0 is_shared))
+    (ensures (fun h0 _ h1 -> sel h0 rp == sel h1 rp)) // the content of rp should stay the same before/ after calling the context
+// TODO: the callback of the program should be able to modify rp
+let progr_passing_callback_test' rp rs f =
+  let secret: ref int = sst_alloc #SNat 0 in
+  sst_encapsulate secret;
+  witness (contains_pred secret); witness (is_encapsulated secret);
+  let cb: elab_typ default_spec (TArr TUnit TUnit) = (fun _ ->
+    recall (contains_pred secret); recall (is_encapsulated secret);
+    sst_write #SNat secret (!secret + 1);
+    raise_val ()) in
+  downgrade_val (f cb);
+  ()
+
 val progr_getting_callback_test:
   rp: ref int ->
   rs: ref (ref int) ->
@@ -280,7 +302,7 @@ val progr_getting_callback_test:
   SST unit
     (requires (fun h0 ->
       satisfy_on_heap rp h0 contains_pred /\
-      ~(is_shared rp h0) /\
+      is_private rp h0 /\
       satisfy_on_heap rs h0 is_shared))
     (ensures (fun h0 _ h1 -> sel h0 rp == sel h1 rp))
 let progr_getting_callback_test rp rs f =
